Examples: Conclude search example

src/panRefinementExampleScript.sml
@@ -122,40 +122,315 @@ Proof
   >> gvs[]
 QED
 
-Proof
-  pan_refinement_tac assign_refinement_rule
-QED
+Definition array_in_mem_def:
+  array_in_mem b l = λs. b <+ b + l ∧ ∀addr. b <=+ addr ∧ addr <+ b + l ⇒ s.memaddrs addr
+End
 
-Theorem assignment_2_step_3:
-  Abbrev (P = var_eq x 0w) ∧
-  Abbrev (Q = postcond (fixed NONE) (var_eq x 10w)) ∧
-  Abbrev (e = (Cmp Less (Var Local x) (Const 10w))) ∧
-  Abbrev (v = (λs. w2n (11w - var_word x s))) ∧
-  Abbrev (i = (λs. ∃w. var_eq x w s ∧ 0w ≤ w ∧ w ≤ 10w)) ⇒
-  refine (WhileC e i v (PanC (Assign Local x (Op Add [(Var Local x); (Const 1w)]))))
-         (PanC (While e (Assign Local x (Op Add [(Var Local x); (Const 1w)]))))
+Theorem clkfree_array_in_mem:
+  ∀b l. clkfree_p (λs. array_in_mem b l s) ∧
+        clkfree_p (array_in_mem b l)
 Proof
-  pan_refinement_thms_tac while_refinement_rule_pan [evaluate_def]
+  rw[clkfree_p_def,array_in_mem_def]
 QED
 
 Definition appears_def:
-  appears x b e = λs. ∃addr. b ≤ addr ∧ addr ≤ e ∧ s.memory addr = x
+  appears x b l = λs. ∃addr. b <=+ addr ∧ addr <+ b + l ∧ s.memory addr = x
 End
 
-Theorem linear_search1:
-  Abbrev (P = (λs. appears x b e s ∧ s.memory = the_mem)) ∧
-  Abbrev (Q = (λ(r,t). r = SOME (Return (ValWord ret)) ∧ b ≤ ret ∧ ret ≤ e ∧ the_mem ret = x)) ⇒
-  refine (HoareC P Q) (DecC v One (Const 0w) (HoareC (set_val P v (Const 0w)) (ignore_val Q v)))
+Theorem clkfree_appears:
+  ∀x b l. clkfree_p (λs. appears x b l s) ∧
+          clkfree_p (appears x b l)
+Proof
+  rw[clkfree_p_def,appears_def]
+QED
+
+Definition mem_eq_def:
+  mem_eq x addr = λs. s.memory addr = x
+End
+
+Theorem clkfree_mem_eq:
+  ∀x addr. clkfree_p (λs. mem_eq x addr s) ∧
+           clkfree_p (mem_eq x addr)
+Proof
+  rw[clkfree_p_def,mem_eq_def]
+QED
+
+Theorem linear_search:
+   v ≠ v2 ⇒
+   refine
+     (HoareC
+        (λs. s.memory = the_mem ∧ array_in_mem b l s ∧ appears (Word x) b l s)
+        (λ(r,t).
+             t.memory = the_mem ∧ array_in_mem b l t ∧
+             ∃ret. r = SOME (Return (ValWord ret)) ∧ b ≤₊ ret ∧ ret <₊ b + l ∧
+                   mem_eq (Word x) ret t))
+     (PanC
+        (Dec v One (Const (0w : word64))
+           (While (Cmp Lower (Var Local v) (Const l))
+              (Dec v2 One (Load One (Op Add [Const b; Var Local v]))
+                 (Seq
+                    (If (Cmp Equal (Var Local v2) (Const x))
+                       (Return (Op Add [Const b; Var Local v])) Skip)
+                    (Assign Local v (Op Add [Const 1w; Var Local v])))))))
 Proof
   rw[]
-  >> irule dec_refinement_rule
-  >> unabbrev_all_tac
+  >> qpat_abbrev_tac ‘P = (λs.
+             s.memory = the_mem ∧ array_in_mem b l s ∧ appears (Word x) b l s)’
+  >> qpat_abbrev_tac ‘Q = (λ(r,t).
+             t.memory = the_mem ∧ array_in_mem b l t ∧
+             ∃ret. r = SOME (Return (ValWord ret)) ∧ b ≤₊ ret ∧ ret <₊ b + l ∧
+                   mem_eq (Word x) ret t)’
+  >> reverse (qsuff_tac ‘refine
+        (HoareC P Q)
+        (DecC v One (Const 0w)
+           (HoareC (λs. P s ∧ var_eq_val Local v (ValWord 0w) s) Q))’)
+  >- (rpt (qpat_x_assum ‘refine _ _’ $ kall_tac)
+      >> pan_refinement_thms_tac dec_refinement_rule_varfree
+                                 [array_in_mem_def,clkfree_array_in_mem,
+                                  appears_def,clkfree_appears,
+                                  mem_eq_def,clkfree_mem_eq])
   >> rw[]
-  >- (gvs[ignore_val_def] >> pairarg_tac >> gvs[])
-  >- (gvs[ignore_val_def] >> pairarg_tac >> gvs[])
-  >- (gvs[ignore_val_def] >> pairarg_tac >> gvs[])
-  >- (gvs[ignore_val_def] >> pairarg_tac >> gvs[])
-  >- (qexists ‘ValWord 0w’ >> gvs[evaluates_to_def,eval_def])
-  >- gvs[appears_def,clkfree_p_def]
-  >- gvs[clkfree_q_def]
+  >> qmatch_asmsub_abbrev_tac ‘DecC v One (Const 0w) (HoareC P' Q)’
+  >> reverse (qsuff_tac ‘refine
+     (HoareC P' Q)
+     (WhileC (Cmp Lower (Var Local v) (Const l))
+        (λs.
+             array_in_mem b l s ∧
+             s.memory = the_mem ∧
+             ∃w. var_eq_val Local v (ValWord w) s ∧ w <₊ l ∧
+                 appears (Word x) (b + w) (l - w) s)
+        (λs. if FLOOKUP s.locals v ≠ NONE then w2n (l - var_word v s) else 0)
+        (HoareC
+           (while_body_pre
+              (λs.
+                   array_in_mem b l s ∧
+                   s.memory = the_mem ∧
+                   ∃w. var_eq_val Local v (ValWord w) s ∧ w <₊ l ∧
+                       appears (Word x) (b + w) (l - w) s)
+              (Cmp Lower (Var Local v) (Const l)))
+           (while_body_post
+              (λs.
+                   array_in_mem b l s ∧
+                   s.memory = the_mem ∧
+                   ∃w. var_eq_val Local v (ValWord w) s ∧ w <₊ l ∧
+                       appears (Word x) (b + w) (l - w) s) (λs. F)
+              (λ(s,r).
+                   ∃ret. r = ValWord ret ∧ b ≤₊ ret ∧ ret <₊ b + l ∧ array_in_mem b l s ∧
+                         s.memory = the_mem ∧ s.memory ret = Word x) (λ(s,eid,e). F))))’)
+  >> qpat_abbrev_tac ‘e = (Cmp Lower (Var Local v) (Const l))’
+  >> qpat_abbrev_tac ‘i = (λs.
+                  array_in_mem b l s ∧
+                  s.memory = the_mem ∧
+                  ∃w. var_eq_val Local v (ValWord w) s ∧ w <₊ l ∧
+                      appears (Word x) (b + w) (l - w) s)’
+  >> qpat_abbrev_tac ‘var = (λs. if FLOOKUP s.locals v ≠ NONE then w2n (l - var_word v s) else 0)’
+  >> qpat_abbrev_tac ‘QB = (λs. F)’
+  >> qpat_abbrev_tac ‘QR = (λ(s,r).
+                        ∃ret. r = ValWord ret ∧ b ≤₊ ret ∧ ret <₊ b + l ∧
+                              array_in_mem b l s ∧ s.memory = the_mem ∧ s.memory ret = Word x)’
+  >> qpat_abbrev_tac ‘QE = (λ(s,eid,e). F)’
+  >- (rpt (qpat_x_assum ‘refine _ _’ $ kall_tac)
+      >> refine_blast_thms_tac while_refinement_rule
+                                 [array_in_mem_def,clkfree_array_in_mem,
+                                  appears_def,clkfree_appears,
+                                  mem_eq_def,clkfree_mem_eq])
+  >> rw[]
+  >> irule refine_transitive
+  >> qexists ‘(DecC v One (Const 0w) (HoareC P' Q))’
+  >> rw[]
+  >> irule refine_transitive
+  >> qexists ‘(DecC v One (Const 0w)
+                 (PanC
+                    (While e
+                       (Dec v2 One (Load One (Op Add [Const b; Var Local v]))
+                          (Seq
+                             (If (Cmp Equal (Var Local v2) (Const x))
+                                (Return (Op Add [Const b; Var Local v])) Skip)
+                             (Assign Local v (Op Add [Const 1w; Var Local v])))))))’
+  >> reverse (rw[])
+  >- gvs[dec_refinement_rule_pan]
+  >> irule refine_monotonic_dec
+  >> irule refine_transitive
+  >> qexists ‘(WhileC e i var
+                      (HoareC (while_body_pre i e) (while_body_post i QB QR QE)))’
+  >> rw[]
+  >> rpt (qpat_x_assum ‘refine _ _’ $ kall_tac)
+  >> qpat_abbrev_tac ‘P'' = while_body_pre i e’
+  >> qpat_abbrev_tac ‘Q' = while_body_post i QB QR QE’
+  >> qpat_abbrev_tac ‘ad = Op Add [Const b; Var Local v]’
+  >> reverse(qsuff_tac ‘refine
+                   (HoareC P'' Q')
+                   (DecC v2 One (Load One ad)
+                      (HoareC (λs. P'' s ∧ var_eq_mem Local v2 ad One s) Q'))’)
+  >- refine_blast_thms_tac dec_refinement_rule_varfree_mem
+                             [array_in_mem_def,clkfree_array_in_mem,
+                              appears_def,clkfree_appears,
+                              mem_eq_def,clkfree_mem_eq]
+  >> qpat_abbrev_tac ‘P'3' = (λs. P'' s ∧ var_eq_mem Local v2 ad One s)’
+  >> rw[]
+  >> reverse(qsuff_tac ‘refine
+                        (HoareC P'3' Q')
+                        (SeqC
+                           (HoareC P'3' (λ(r,t).
+                                                 if r ≠ NONE then Q'(r,t)
+                                                 else (λs.
+                                                         P'3' s ∧
+                                                         FLOOKUP s.locals v2 ≠ SOME (ValWord x) ∧
+                                                         ∃w. FLOOKUP s.locals v = SOME (ValWord w) ∧
+                                                             w + 1w <₊ l) t))
+                           (HoareC (λs.
+                                        P'3' s ∧
+                                        FLOOKUP s.locals v2 ≠ SOME (ValWord x) ∧
+                                        ∃w. FLOOKUP s.locals v = SOME (ValWord w) ∧ w + 1w <₊ l) Q'))’)
+  >> qpat_abbrev_tac ‘M = (λs. P'3' s ∧ FLOOKUP s.locals v2 ≠ SOME (ValWord x) ∧
+                               ∃w. FLOOKUP s.locals v = SOME (ValWord w) ∧ w + 1w <₊ l)’
+  >- (rpt (qpat_x_assum ‘refine _ _’ $ kall_tac)
+      >> pan_refinement_thms_tac seq_refinement_rule_both
+                             [array_in_mem_def,clkfree_array_in_mem,
+                              appears_def,clkfree_appears,
+                              mem_eq_def,clkfree_mem_eq])
+  >> qpat_abbrev_tac ‘Q'' = (λ(r,t). if r ≠ NONE then Q' (r,t) else M t)’
+  >> rw[]
+  >> reverse(qsuff_tac ‘refine
+                        (HoareC P'3' Q'')
+                        (IfC (Cmp Equal (Var Local v2) (Const x))
+                           (HoareC
+                              (λs. P'3' s ∧ evaluates_to_true (Cmp Equal (Var Local v2) (Const x)) s)
+                              Q'')
+                           (HoareC
+                              (λs. P'3' s ∧ evaluates_to_false (Cmp Equal (Var Local v2) (Const x)) s)
+                              Q''))’)
+  >> qpat_abbrev_tac ‘e' = (Cmp Equal (Var Local v2) (Const x))’
+  >- (rpt (qpat_x_assum ‘refine _ _’ $ kall_tac)
+      >> pan_refinement_thms_tac if_refinement_rule
+                             [array_in_mem_def,clkfree_array_in_mem,
+                              appears_def,clkfree_appears,
+                              mem_eq_def,clkfree_mem_eq])
+  >> qpat_abbrev_tac ‘P'4' = (λs. P'³' s ∧ evaluates_to_true e' s)’
+  >> qpat_abbrev_tac ‘P'5' = (λs. P'³' s ∧ evaluates_to_false e' s)’
+  >> rw[]
+  >> reverse(qsuff_tac ‘refine (HoareC P'4' Q'') (PanC (Return ad))’)
+  >- (rpt(qpat_x_assum ‘refine _ _’ $ kall_tac)
+      >> refine_blast_thms_tac return_refinement_rule
+                             [array_in_mem_def,clkfree_array_in_mem,
+                              appears_def,clkfree_appears,
+                              mem_eq_def,clkfree_mem_eq])
+  >> rw[]
+  >> dxrule_all_then assume_tac (cj 1 refine_monotonic_if)
+  >> first_x_assum $ qspecl_then [‘HoareC P'5' Q''’, ‘e'’] assume_tac
+  >> dxrule_all_then assume_tac refine_transitive
+  >> reverse(qsuff_tac ‘refine (HoareC P'5' Q'') (PanC (Skip))’)
+  >- (rpt(qpat_x_assum ‘refine _ _’ $ kall_tac)
+      >> pan_refinement_thms_tac skip_refinement_rule
+                             [array_in_mem_def,clkfree_array_in_mem,
+                              appears_def,clkfree_appears,
+                              mem_eq_def,clkfree_mem_eq]
+      >> first_x_assum $ mp_tac
+      >> gvs[]
+      >> Cases_on ‘b + c' = addr’
+      >> gvs[]
+      >> blast_tac)
+  >> rw[]
+  >> dxrule_all_then assume_tac (cj 2 refine_monotonic_if)
+  >> first_x_assum $ qspecl_then [‘PanC (Return ad)’, ‘e'’] assume_tac
+  >> dxrule_all_then assume_tac refine_transitive
+  >> reverse(qsuff_tac ‘refine (IfC e' (PanC (Return ad)) (PanC Skip)) (PanC (If e' (Return ad) Skip))’)
+  >- (gvs[if_refinement_rule_pan])
+  >> rw[]
+  >> dxrule_all_then assume_tac refine_transitive
+  >> dxrule_all_then assume_tac (cj 1 refine_monotonic_seq)
+  >> first_x_assum $ qspec_then ‘HoareC M Q'’ assume_tac
+  >> reverse(qsuff_tac ‘refine (HoareC M Q') (PanC (Assign Local v (Op Add [Const 1w; Var Local v])))’)
+  >- (rpt(qpat_x_assum ‘refine _ _’ $ kall_tac)
+      >> pan_refinement_thms_tac assign_refinement_rule
+                             [array_in_mem_def,clkfree_array_in_mem,
+                              appears_def,clkfree_appears,
+                              mem_eq_def,clkfree_mem_eq]
+      >> first_x_assum $ mp_tac
+      >> gvs[]
+      >> Cases_on ‘b + c = addr’
+      >> gvs[]
+      >> blast_tac)
+  >> rw[]
+  >> dxrule_all_then assume_tac (cj 2 refine_monotonic_seq)
+  >> first_x_assum $ qspec_then ‘(PanC (If e' (Return ad) Skip))’ assume_tac
+  >> dxrule_all_then assume_tac refine_transitive
+  >> reverse(qsuff_tac ‘refine
+                        (SeqC
+                           (PanC (If e' (Return ad) Skip))
+                           (PanC (Assign Local v (Op Add [Const 1w; Var Local v]))))
+                        (PanC (Seq (If e' (Return ad) Skip)
+                                   (Assign Local v (Op Add [Const 1w; Var Local v]))))’)
+  >- gvs[seq_refinement_rule_pan]
+  >> rw[]
+  >> qspecl_then [‘HoareC P'3' Q'’, ‘SeqC (HoareC P'³' Q'') (HoareC M Q')’,
+                  ‘v2’, ‘One’, ‘Load One ad’] assume_tac refine_monotonic_dec
+  >> gvs[]
+  >> dxrule_all_then assume_tac refine_transitive
+  >> dxrule_all_then assume_tac refine_monotonic_dec
+  >> first_x_assum $ qspecl_then [‘v2’, ‘One’, ‘Load One ad’] assume_tac
+  >> dxrule_all_then assume_tac refine_transitive
+  >> reverse(qsuff_tac ‘refine
+                        (DecC v2 One (Load One ad)
+                           (PanC
+                              (Seq (If e' (Return ad) Skip)
+                                  (Assign Local v (Op Add [Const 1w; Var Local v])))))
+                        (PanC
+                            (Dec v2 One (Load One ad)
+                               (Seq (If e' (Return ad) Skip)
+                                   (Assign Local v (Op Add [Const 1w; Var Local v])))))’)
+  >- gvs[dec_refinement_rule_pan]
+  >> rw[]
+  >> dxrule_all_then assume_tac refine_transitive
+  >> dxrule_all_then assume_tac refine_transitive
+  >> dxrule_all_then assume_tac refine_monotonic_while
+  >> first_x_assum $ qspecl_then [‘e’, ‘i’, ‘var’] assume_tac
+  >> irule refine_transitive
+  >> qexists ‘(WhileC e i var
+             (PanC
+                (Dec v2 One (Load One ad)
+                   (Seq (If e' (Return ad) Skip)
+                        (Assign Local v (Op Add [Const 1w; Var Local v]))))))’
+  >> rw[]
+  >> rpt (qpat_x_assum ‘refine _ _’ $ kall_tac)
+  >> irule while_refinement_rule_pan
+  >> unabbrev_all_tac
+  >> gvs[array_in_mem_def,appears_def,mem_eq_def,var_eq_val_def]
+  >> rw[is_variant_def]
+  >> BasicProvers.every_case_tac
+  >> gvs[]
+  >- (‘0w <₊ w - l’ by blast_tac
+      >> Cases_on ‘w2n (l + -1w * w)’
+      >> gvs[]
+      >> blast_tac)
+  >> first_x_assum $ mp_tac
+  >> rw_tac pan_refinement_ss [evaluate_def]
+  >- (Cases_on ‘s.memory (b + w)’
+      >> gvs[]
+      >> Cases_on ‘c' = x’
+      >> gvs[]
+      >- (gvs[evaluate_def,eval_def,wordLangTheory.word_op_def,finite_mapTheory.FLOOKUP_UPDATE,
+              size_of_shape_def,shape_of_def,empty_locals_def]
+          >> Cases_on ‘FLOOKUP s.locals v2’
+          >> gvs[res_var_def,finite_mapTheory.FLOOKUP_UPDATE])
+      >> gvs[evaluate_def,finite_mapTheory.FLOOKUP_UPDATE,shape_of_def]
+      >> Cases_on ‘FLOOKUP s.locals v2’
+      >> gvs[res_var_def,finite_mapTheory.FLOOKUP_UPDATE,finite_mapTheory.DOMSUB_FLOOKUP_THM]
+      >> blast_tac)
+  >- (spose_not_then assume_tac
+      >> qpat_x_assum ‘¬_’ $ mp_tac
+      >> gvs[]
+      >> first_x_assum $ irule
+      >> blast_tac)
+  >> Cases_on ‘s.memory (b + w)’
+  >> gvs[]
+  >> Cases_on ‘c = x’
+  >> gvs[]
+  >- (gvs[evaluate_def,eval_def,wordLangTheory.word_op_def,finite_mapTheory.FLOOKUP_UPDATE,
+          size_of_shape_def,shape_of_def,empty_locals_def]
+      >> Cases_on ‘FLOOKUP s.locals v2’
+      >> gvs[res_var_def,finite_mapTheory.FLOOKUP_UPDATE])
+  >> gvs[evaluate_def,finite_mapTheory.FLOOKUP_UPDATE,shape_of_def]
+  >> Cases_on ‘FLOOKUP s.locals v2’
+  >> gvs[res_var_def,finite_mapTheory.FLOOKUP_UPDATE,finite_mapTheory.DOMSUB_FLOOKUP_THM]
 QED
